Tried to replace reveal by showing the property with pkenc_input but failed

src/lib/communication/DY.Lib.Communication.Core.Invariants.fst
@@ -16,16 +16,29 @@ open DY.Lib.Communication.Core
 
 (*** PkEnc Predicates ***)
 
+#push-options "--ifuel 3 --fuel 0"
 val pkenc_crypto_predicates_communication_layer: {|cusages:crypto_usages|} -> pkenc_crypto_predicate
 let pkenc_crypto_predicates_communication_layer #cusages = {
-  pred = (fun tr sk_usage pk msg ->
-    (exists sender receiver.
+  pred = (fun tr sk_usage msg ->
+    match parse pkenc_input msg with
+    | Some (PkEncInput payload) -> (
+      (exists sender receiver.
+        sk_usage == long_term_key_type_to_usage (LongTermPkEncKey comm_layer_pkenc_tag)  receiver /\
+        (get_label tr payload) `can_flow tr` (join (principal_label sender) (principal_label receiver)) /\
+        event_triggered tr sender (CommConfSendMsg sender receiver payload)
+      )
+    )
+    | Some (PkEncSignInput {sender; receiver; payload}) -> (
       sk_usage == long_term_key_type_to_usage (LongTermPkEncKey comm_layer_pkenc_tag)  receiver /\
-      (get_label tr msg) `can_flow tr` (join (principal_label sender) (principal_label receiver)) /\
-      event_triggered tr sender (CommConfSendMsg sender receiver msg)
-    ));
-  pred_later = (fun tr1 tr2 sk_usage pk msg -> ());
+      (get_label tr payload) `can_flow tr` (join (principal_label sender) (principal_label receiver)) /\
+      event_triggered tr sender (CommConfSendMsg sender receiver payload) /\
+      event_triggered tr sender (CommConfAuthSendMsg sender receiver payload)
+    )
+    | None -> False
+    );
+  pred_later = (fun tr1 tr2 pk msg -> parse_wf_lemma pkenc_input (bytes_well_formed tr1) msg);
 }
+#pop-options
 
 val pkenc_crypto_predicates_communication_layer_and_tag: 
   {|cusages:crypto_usages|} ->
@@ -35,7 +48,24 @@ let pkenc_crypto_predicates_communication_layer_and_tag #cusages =
 
 (*** Sign Predicates ***)
 
-#push-options "--ifuel 3 --fuel 0"
+(*
+val pk_enc_extract_msg: enc_msg:bytes{exists pk nonce msg. enc_msg = pk_enc pk nonce msg} -> GTot (msg:bytes{exists pk nonce. enc_msg = pk_enc pk nonce msg})
+let pk_enc_extract_msg enc_msg =
+  normalize_term_spec pk_enc;
+  match enc_msg with
+  | DY.Core.Bytes.Type.PkEnc pk nonce msg -> msg
+
+val pk_enc_extract_sk: enc_msg:bytes -> option bytes
+let pk_enc_extract_sk enc_msg =
+  match enc_msg with
+  | DY.Core.Bytes.Type.PkEnc pk nonce msg -> (
+    match pk with
+    | DY.Core.Bytes.Type.Pk sk -> Some sk
+    | _ -> None
+  )
+  | _ -> None*)
+
+#push-options "--ifuel 4 --fuel 4 --z3rlimit 50"
 val sign_crypto_predicates_communication_layer: {|cusages:crypto_usages|} -> sign_crypto_predicate
 let sign_crypto_predicates_communication_layer #cusages = {
   pred = (fun tr sk_usage vk sig_msg ->
@@ -45,18 +75,27 @@ let sign_crypto_predicates_communication_layer #cusages = {
       get_label tr payload `can_flow tr` public /\
       event_triggered tr sender (CommAuthSendMsg sender payload)
     )
-    | Some (Encrypted {sender; receiver; payload=enc_payload}) -> (
-      match pk_enc_extract_msg enc_payload with
-      | None -> False
-      | Some plain_payload -> (
-        sk_usage == long_term_key_type_to_usage (LongTermSigKey comm_layer_sign_tag) sender /\     
-        get_label tr enc_payload `can_flow tr` public /\
-        event_triggered tr sender (CommConfAuthSendMsg sender receiver plain_payload)
+    | Some (Encrypted payload) -> (  
+      get_label tr payload `can_flow tr` public /\
+
+      (exists (plain_payload:communication_message) nonce pk_receiver.
+        sk_usage == long_term_key_type_to_usage (LongTermSigKey comm_layer_sign_tag) plain_payload.sender /\
+
+        //pk_enc_extract_pk enc_payload == Some (DY.Core.Bytes.Type.Pk sk_receiver) /\
+        //Some plain_msg == decrypt_message sk_receiver enc_payload /\
+        //get_label sk_receiver == principal_label receiver /\
+        bytes_well_formed tr pk_receiver /\
+        pk_receiver `has_sk_usage tr` (long_term_key_type_to_usage (LongTermPkEncKey comm_layer_pkenc_tag) plain_payload.receiver) /\
+        payload == encrypt_message pk_receiver nonce (PkEncSignInput plain_payload) /\
+        //event_triggered tr sender (CommConfSendMsg sender receiver plain_msg) /\
+        //event_triggered tr sender (CommAuthSendMsg sender plain_msg) /\
+        event_triggered tr plain_payload.sender (CommConfAuthSendMsg plain_payload.sender plain_payload.receiver plain_payload.payload) //\
+        //get_label plain_msg `can_flow tr` (join (principal_label sender) (principal_label receiver))
       )
     )
     | None -> False)
   );
-  pred_later = (fun tr1 tr2 sk_usage vk msg ->  parse_wf_lemma signature_input (bytes_well_formed tr1) msg);
+  pred_later = (fun tr1 tr2 sk_usage msg -> parse_wf_lemma signature_input (bytes_well_formed tr1) msg);
 }
 #pop-options
 
